lvars/coq/Spec.v
@@ -1,8 +1,9 @@
 Require Export List.
 Export ListNotations.
 Require Import Coq.Program.Equality. 
-Require Export Heap. 
-Require Export AST. 
+Require Import Heap. 
+Require Import AST. 
+Require Import NonSpec.  
 
 
 Inductive pool : Type :=
@@ -10,13 +11,13 @@ Inductive pool : Type :=
   |dot : pool
   |par : pool -> pool -> pool.
 
+Hint Constructors pool. 
+
 Fixpoint bump (t : tid) : tid := 
   match t with
     |(maj, min) :: t' => (maj, S min) :: t'
     |nil => nil
   end.
-
-Open Scope list_scope.
  
 Inductive congr : pool -> pool -> Prop :=
   |comm : forall t1 t2, congr (par t1 t2) (par t2 t1)
@@ -24,7 +25,9 @@ Inductive congr : pool -> pool -> Prop :=
   |refl : forall t1, congr t1 t1
 .
 
+Hint Constructors congr. 
 
+Definition sHeap := heap (ivar_state). 
 
 Inductive ctxt : (term -> term) -> Prop :=
 |bindCtxt : forall N c, ctxt c -> ctxt (fun M => bind (c M) N)
@@ -32,13 +35,14 @@ Inductive ctxt : (term -> term) -> Prop :=
 |handleCtxt : forall N c, ctxt c -> ctxt (fun M => handle M N)
 |hole : forall c, ctxt c -> ctxt (fun M => c M)
 .
+Hint Constructors ctxt. 
 
-Inductive rollback : tid -> heap -> pool -> heap -> pool -> Prop :=
-|RBDone : forall t maj min h min' M' tid' M T s2, 
+Inductive rollback : tid -> sHeap -> pool -> sHeap -> pool -> Prop :=
+|RBDone : forall T t maj min h min' M' tid' M s2, 
             rollback ((maj, min)::t) h (par (thread ((maj, min') :: t) [sAct tid' M'] s2 M) T)
                      h (par (thread ((maj, min') :: t) [sAct tid' M'] s2 M) T)
 |RBRead : forall s1 s1' s2 x tid tid' tid'' M M' N h h' h'' T T' sc t A S ds, 
-            s1 = s1' ++ [rAct x tid'' M'] -> heap_lookup x h = full sc (tid''::ds) (S::A) t N ->
+            s1 = s1' ++ [rAct x tid'' M'] -> heap_lookup x h = Some (full sc (tid''::ds) (S::A) t N) ->
             h' = replace x (full sc ds (S::A) t N) h -> 
             rollback tid h' (par (thread tid'' s1' s2 M') T) h'' T'->
             rollback tid h (par(thread tid' s1 s2 M) T) h'' T'
@@ -47,12 +51,12 @@ Inductive rollback : tid -> heap -> pool -> heap -> pool -> Prop :=
             rollback tid h (par (thread tid'' s1' s2 M') T) h' T' ->
             rollback tid h (par (par (thread tid' s1 s2 M) (thread tid'' [specAct] s2' N)) T) h' T'
 |RBWrite : forall s1 s1' s2 tid tid' tid'' M M' N S A sc T T' h h' h'' x,
-             s1 = s1' ++ [wAct x tid'' M'] -> heap_lookup x h = full sc nil (S::A) tid'' N ->
+             s1 = s1' ++ [wAct x tid'' M'] -> heap_lookup x h = Some(full sc nil (S::A) tid'' N) ->
              h' = replace x (empty sc) h -> 
              rollback tid h' (par (thread tid'' s1' s2 M') T) h'' T' ->
              rollback tid h (par (thread tid' s1 s2 M) T) h'' T'
 |RBNew : forall s1 s1' s2 tid tid' tid'' M M' S A T T' h h' h'' x,
-           s1 = s1' ++ [cAct x tid'' M'] -> heap_lookup x h = empty (S::A) ->
+           s1 = s1' ++ [cAct x tid'' M'] -> heap_lookup x h = Some (empty (S::A)) ->
            h' = remove h x -> 
            rollback tid h' (par (thread tid'' s1' s2 M') T) h'' T' ->
            rollback tid h (par (thread tid' s1 s2 M) T) h'' T'
@@ -61,12 +65,18 @@ Inductive rollback : tid -> heap -> pool -> heap -> pool -> Prop :=
             rollback tid h (par (thread tid'' s1' s2 M') T) h' T' ->
             rollback tid h (par (par (thread tid' s1 s2 M) 
                                              (thread tid''' [sAct tid2 N'; specAct] s2' N)) T) h' T'
+(*
+|RBComm : forall tid h h' T1 T2 T',
+            rollback tid h (par T2 T1) h' T' ->
+            rollback tid h (par T1 T2) h' T'
+.*)
 |RBCongr : forall tid h h' T T' T'' T''', 
              congr T T' -> congr T'' T''' -> rollback tid h T' h' T'' ->
              rollback tid h T h' T'''
 .
 
-Inductive step : heap -> pool -> heap -> pool -> Prop :=
+Hint Constructors rollback. 
+Inductive step : sHeap -> pool -> sHeap -> pool -> Prop :=
 |Bind : forall t1 t2 h s1 s2 tid E T M,
            ctxt E -> M = E (bind (ret t1) t2) ->
            step h (par (thread tid s1 s2 M) T) h (par (thread (bump tid) s1 s2 (E (app t2 t1))) T)
@@ -79,12 +89,12 @@ Inductive step : heap -> pool -> heap -> pool -> Prop :=
                (par (par (thread (bump tid) (fAct ((1,1)::tid) tid M :: s1) s2 (ret unit))
                          (thread ((1, 1)::tid) nil nil M')) T)
 |Get : forall E M x h sc (ds : list tid) s t N h' T s1 s2 ds tid,
-         ctxt E -> M = E (get x) -> heap_lookup x h = full sc ds s t N -> 
+         ctxt E -> M = E (get x) -> heap_lookup x h = Some(full sc ds s t N) -> 
          h' = replace x (full sc (tid::ds) s t N) h->
          step h (par (thread tid s1 s2 M) T) h' 
               (par (thread (bump tid) (rAct x tid M :: s1) s2 (E(ret N))) T)
 |Put : forall E M x N h sc h' s1 s2 tid T ,
-         ctxt E -> M = E (put x N) -> heap_lookup x h = empty sc ->
+         ctxt E -> M = E (put x N) -> heap_lookup x h = Some(empty sc) ->
          h' = replace x (full sc nil s1 tid N) h ->
          step h (par (thread tid s1 s2 M) T) h' 
               (par (thread (bump tid) (wAct x tid M::s1) s2 (E(ret unit))) T)
@@ -121,20 +131,24 @@ Inductive step : heap -> pool -> heap -> pool -> Prop :=
 |Handle : forall h tid s1 s2 M N T c E,
             ctxt c -> M = c (handle (raise E) N) ->
             step h (par (thread tid s1 s2 M) T) h (par (thread (bump tid) s1 s2 (c (app N E))) T)
+|HandleRet : forall h tid s1 s2 M N T c M',
+               ctxt c -> M = c(handle(ret M') N) ->
+               step h (par (thread tid s1 s2 M) T) h 
+                    (par (thread (bump tid) s1 s2 (c (ret M'))) T)
 |PopRead : forall h tid tid' s1 s1' s2 M M' i ds t N,
-             s1 = s1' ++ [rAct i tid' M'] -> heap_lookup i h = full nil ds nil t N ->
+             s1 = s1' ++ [rAct i tid' M'] -> heap_lookup i h = Some(full nil ds nil t N) ->
              step h (thread tid s1 s2 M) h (thread (bump tid) s1' ((rAct i tid' M')::s2) M)
 |PopWrite : forall h tid tid' s1 s1' s2 M' M ds s N i,
-              s1 = s1' ++ [wAct i tid' M'] -> heap_lookup i h = full nil ds s tid' N ->
+              s1 = s1' ++ [wAct i tid' M'] -> heap_lookup i h = Some(full nil ds s tid' N) ->
               step h (thread tid s1 s2 M) (replace i (full nil nil nil tid' N) h)
                    (thread (bump tid) s1' ((wAct i tid' M') :: s2) M)
 |PopNewFull : forall h h' s1 s1' s2 i tid tid' M' ds s s' t M N T, 
-                s1 = s1' ++ [cAct i tid' M'] -> heap_lookup i h = full s ds s' t N ->
+                s1 = s1' ++ [cAct i tid' M'] -> heap_lookup i h = Some(full s ds s' t N) ->
                 h' = replace i (full nil ds s' t N) h -> 
                 step h (par (thread tid s1 s2 M) T) h'
                      (par (thread tid s1' ((cAct i tid' M')::s2) M) T)
 |PopNewEmpty : forall h h' s1 s1' s2 i tid tid' M' s M T, 
-                 s1 = s1' ++ [cAct i tid' M'] -> heap_lookup i h = empty s ->
+                 s1 = s1' ++ [cAct i tid' M'] -> heap_lookup i h = Some(empty s) ->
                  h' = replace i (empty nil) h ->
                  step h (par (thread tid s1 s2 M) T) h'
                       (par (thread tid s1' ((cAct i tid' M')::s2) M) T)
@@ -143,10 +157,14 @@ Inductive step : heap -> pool -> heap -> pool -> Prop :=
              step h (par (par (thread tid s1 s2 M) (thread tid' s1'' s2' N)) T)
                   h (par (par (thread (bump tid) s1' ((fAct tid1 tid2 M')::s2) M) 
                               (thread (bump tid') s1''' (specAct :: s2') N)) T)
-|Terminate : forall h tid s M T, step h (par (thread tid nil s (ret M)) T) h T
-|CongrStep : forall t1 t1' t2 t2' h h', congr t1 t1' -> congr t2 t2' -> step h t1' h' t2' ->
-                                        step h t1 h' t2
+|Terminate : forall h tid s M T, step h (par (thread tid nil s (ret M)) T) h 
+                                        (par dot T)
+|CongrStep : forall t1 t1' t2 t2' h h', 
+               step h t1' h' t2' -> congr t1 t1' -> congr t2 t2' ->
+               step h t1 h' t2
 .
+
+Hint Constructors step. 
 
 Tactic Notation "step_cases" tactic(first) ident(c) :=
   first;
@@ -159,15 +177,24 @@ Tactic Notation "step_cases" tactic(first) ident(c) :=
     Case_aux c "Terminate" | Case_aux c "CongrStep"
 ].
 
-Inductive unspecHeap : heap -> heap -> Prop :=
-  |unSpecSE : forall h h' i hd tl, unspecHeap h h' -> unspecHeap ((i, empty (hd::tl)) :: h') h'
-  |unSpecCE : forall h h' i, unspecHeap h h' -> unspecHeap ((i, empty nil) :: h') ((i, empty nil) :: h')
-  |unspecSF : forall h h' i hd tl d s t N, unspecHeap h h' -> unspecHeap ((i, full (hd::tl) d s t N) :: h') h'
-  |unspecCCSF : forall h h' i d hd tl t M, unspecHeap h h' ->
-                                           unspecHeap ((i, full nil d (hd::tl) t M)::h) ((i, empty nil)::h')
-  |unspecCCCF : forall h h' i d t M, unspecHeap h h' ->
-                                     unspecHeap ((i, full nil d nil t M)::h) ((i, full nil d nil t M)::h')
+Inductive unspecHeap : sHeap -> sHeap -> Prop :=
+  |unSpecSE : forall h h' i hd tl, unspecHeap h h' -> 
+                                   unspecHeap ((i, empty (hd::tl)) :: h) h'
+  |unSpecCE : forall h h' i, unspecHeap h h' -> 
+                             unspecHeap ((i, empty nil) :: h) ((i, empty nil) :: h')
+  |unspecSF : forall h h' i hd tl d s t N, 
+                unspecHeap h h' -> 
+                unspecHeap ((i, full (hd::tl) d s t N) :: h) h'
+  |unspecCCSF : forall h h' i d hd tl t M, 
+                  unspecHeap h h' ->
+                  unspecHeap ((i, full nil d (hd::tl) t M)::h) ((i, empty nil)::h')
+  |unspecCCCF : forall h h' i d t M, 
+                  unspecHeap h h' ->
+                  unspecHeap ((i, full nil d nil t M)::h) 
+                             ((i, full nil d nil t M)::h')
 .
+
+Hint Constructors unspecHeap. 
 
 Inductive unspecT : pool -> pool -> Prop :=
   |unSpecDot : unspecT dot dot
@@ -175,36 +202,47 @@ Inductive unspecT : pool -> pool -> Prop :=
                  unspecT t1 t1' -> unspecT t2 t2' -> unspecT (par t1 t2) (par t1' t2')
   |unSpecCThread : forall tid s2 M,
                     unspecT (thread tid nil s2 M) (thread tid nil s2 M)
-  |unSpecRead : forall tid s1 s1' s2 M i tid' M',
-                  s1 = s1' ++ [rAct i tid' M'] -> 
-                  unspecT (thread tid s1 s2 M) (thread tid' nil s2 M')
-  |unSpecWrite : forall tid s1 s1' s2 M i tid' M',
-                   s1 = s1' ++ [wAct i tid' M'] ->
-                   unspecT (thread tid s1 s2 M) (thread tid' nil s2 M')
-  |unSpecCreate : forall tid s1 s1' s2 M i tid' M',
-                  s1 = s1' ++ [cAct i tid' M'] ->
-                  unspecT (thread tid s1 s2 M) (thread tid' nil s2 M')
-  |unSpecSpec : forall tid s1 s1' s2 M tid' M',
-                  s1 = s1' ++ [sAct tid' M'] ->
-                  unspecT (thread tid s1 s2 M) (thread tid' [sAct tid' M'] s2 M')
-  |unSpecFork : forall tid s1 s1' s2 M tid' M' tid'',
-                  s1 = s1' ++ [fAct tid' tid'' M'] ->
-                  unspecT (thread tid s1 s2 M) (thread tid'' nil s2 M').
+  |unSpecRead : forall tid s1 s1' s2 M i M' maj min min',
+                  s1 = s1' ++ [rAct i ((maj, min')::tid) M'] -> 
+                  unspecT (thread ((maj, min)::tid) s1 s2 M) 
+                          (thread ((maj, min')::tid) nil s2 M')
+  |unSpecWrite : forall tid s1 s1' s2 M i M' maj min min',
+                   s1 = s1' ++ [wAct i ((maj, min')::tid) M'] ->
+                   unspecT (thread ((maj, min)::tid) s1 s2 M) 
+                           (thread ((maj, min')::tid) nil s2 M')
+  |unSpecCreate : forall tid s1 s1' s2 M i maj min min' M',
+                  s1 = s1' ++ [cAct i ((maj, min')::tid) M'] ->
+                  unspecT (thread ((maj, min)::tid) s1 s2 M) 
+                          (thread ((maj, min')::tid) nil s2 M')
+  |unSpecSpec : forall tid s1 s1' s2 M maj min min' M',
+                  s1 = s1' ++ [sAct ((maj, min')::tid) M'] ->
+                  unspecT (thread ((maj, min)::tid) s1 s2 M) 
+                          (thread ((maj, min')::tid) [sAct ((maj, min')::tid) M'] s2 M')
+  |unSpecFork : forall tid s1 s1' s2 M tid' M' maj min min',
+                  s1 = s1' ++ [fAct tid' ((maj, min')::tid) M'] ->
+                  unspecT (thread ((maj, min)::tid) s1 s2 M) 
+                          (thread ((maj, min')::tid) nil s2 M').
+Hint Constructors unspecT. 
 
 
-Inductive unspec : heap -> pool -> heap -> pool -> Prop :=
+Inductive unspec : sHeap -> pool -> sHeap -> pool -> Prop :=
   |Unspec : forall h h' p p', unspecHeap h h' -> unspecT p p' -> unspec h p h' p'.
 
+Hint Constructors unspec. 
 
-Inductive multistep : heap -> pool -> heap -> pool -> Prop :=
+Inductive multistep : sHeap -> pool -> sHeap -> pool -> Prop :=
 |reflStep : forall h p, multistep h p h p
 |multiStep : forall h h' h'' p p' p'', step h p h' p' -> multistep h' p' h'' p'' ->
                                multistep h p h'' p''
 .
 
-Inductive wellFormed : heap -> pool -> Prop :=
+Hint Constructors multistep. 
+
+Inductive wellFormed : sHeap -> pool -> Prop :=
 |WF : forall h h' p p', unspecHeap h h' -> unspecT p p' -> multistep h' p' h p ->
                         wellFormed h p.
+
+Hint Constructors wellFormed. 
 
 Inductive specActions : pool -> list (tid * specStack) -> Prop :=
   |sCompActions : forall T1 T2 a1 a2, specActions T1 a1 -> specActions T2 a2 ->
@@ -214,6 +252,8 @@ Inductive specActions : pool -> list (tid * specStack) -> Prop :=
   |sDotActions : specActions dot nil
 .
 
+Hint Constructors specActions. 
+
 Inductive commitActions : pool -> list (tid * specStack) -> Prop :=
   |nsCompActions : forall T1 T2 a1 a2, commitActions T1 a1 -> commitActions T2 a2 ->
                                        commitActions (par T1 T2) (a1 ++ a2)
@@ -221,7 +261,248 @@ Inductive commitActions : pool -> list (tid * specStack) -> Prop :=
                        commitActions (thread ((maj, min)::tid) s1 s2 M) [((maj, 1)::tid, s2)]
   |nsDotActions : commitActions dot nil
 .
+Hint Constructors commitActions. 
+
+
+Inductive thread_lookup : pool -> tid -> option pool -> Prop :=
+|hit : forall tid maj min min' s1 s2 M,
+         thread_lookup (thread ((maj, min)::tid) s1 s2 M) ((maj, min')::tid) 
+                       (Some (thread ((maj, min)::tid) s1 s2 M))
+|miss : forall tid maj min tid' maj' min' s1 s2 M,
+          tid <> tid' \/ maj <> maj' ->
+          thread_lookup (thread ((maj, min)::tid) s1 s2 M) ((maj', min')::tid') 
+                        None
+|lookupPar : forall T1 T2 tid T, 
+               thread_lookup T1 tid (Some T) -> thread_lookup (par T1 T2) tid (Some T)
+|lookupPar2 : forall T1 T2 tid T,
+                thread_lookup T1 tid None -> thread_lookup T2 tid T ->
+                thread_lookup (par T1 T2) tid T
+|lookupDot : forall tid, thread_lookup dot tid None
+.
+
+Hint Constructors thread_lookup. 
+
+(*Erasure*)
+Inductive appears_free_in : id -> term -> Prop :=
+|afi_ivar : forall i j, i <> j -> appears_free_in i (ivar j)
+|afi_unit : forall i, appears_free_in i unit
+|afi_pair : forall i e1 e2, appears_free_in i e1 -> appears_free_in i e2 ->
+                            appears_free_in i (pair e1 e2)
+|afi_var : forall i j, i <> j -> appears_free_in i (var j)
+|afi_lambda : forall i j e, i <> j -> appears_free_in i e -> 
+                            appears_free_in i (lambda j e)
+|afi_app : forall i e1 e2, appears_free_in i e1 -> appears_free_in i e2 ->
+                           appears_free_in i (app e1 e2)
+|afi_ret : forall i e, appears_free_in i e -> appears_free_in i (ret e)
+|afi_bind : forall i e1 e2, appears_free_in i e1 -> appears_free_in i e2 ->
+                            appears_free_in i (bind e1 e2)
+|afi_fork : forall i e, appears_free_in i e -> appears_free_in i (fork e)
+|afi_new : forall i, appears_free_in i new
+|afi_put : forall i j e, appears_free_in i e -> appears_free_in i (put j e)
+|afi_get : forall i j, appears_free_in i (get j)
+|afi_raise : forall i e, appears_free_in i e -> appears_free_in i (raise e)
+|afi_handle : forall i e1 e2, appears_free_in i e1 -> appears_free_in i e2 ->
+                              appears_free_in i (handle e1 e2)
+|afi_done : forall i e, appears_free_in i e -> appears_free_in i (done e)
+|afi_spec : forall i e1 e2, appears_free_in i e1 -> appears_free_in i e2 ->
+                            appears_free_in i (spec e1 e2)
+|afi_spec_return : forall i e1 e2, appears_free_in i e1 -> appears_free_in i e2 ->
+                                   appears_free_in i (specReturn e1 e2)
+.
+
+Hint Constructors appears_free_in. 
+
+Inductive eraseTerm : term -> pool -> pterm -> Prop :=
+|eraseIVar : forall i T, eraseTerm (ivar i) T (pivar i)
+|eraseUnit : forall T, eraseTerm unit T punit
+|erasePair : forall t1 t1' t2 t2' T, eraseTerm t1 T t1' -> eraseTerm t2 T t2' ->
+                                     eraseTerm (pair t1 t2) T (ppair t1' t2')
+|eraseVar : forall i T, eraseTerm (var i) T (pvar i)
+|eraseLambda : forall i e e' T, eraseTerm e T e' -> 
+                                eraseTerm (lambda i e) T (plambda i e')
+|eraseApp : forall e1 e1' e2 e2' T, eraseTerm e1 T e1' -> eraseTerm e2 T e2' ->
+                                    eraseTerm (app e1 e2) T (papp e1' e2')
+|eraseRet : forall e e' T, eraseTerm e T e' -> eraseTerm (ret e) T (pret e')
+|eraseBind : forall e1 e1' e2 e2' T, eraseTerm e1 T e1' -> eraseTerm e2 T e2' ->
+                                     eraseTerm (bind e1 e2) T (pbind e1' e2')
+|eraseFork : forall e e' T, eraseTerm e T e' -> eraseTerm (fork e) T (pfork e')
+|eraseNew : forall T, eraseTerm new T pnew
+|erasePut : forall e e' i T, eraseTerm e T e' -> eraseTerm (put i e) T (pput i e')
+|eraseGet : forall i T, eraseTerm (get i) T (pget i)
+|eraseRaise : forall e e' T, eraseTerm e T e' -> eraseTerm (raise e) T (praise e')
+|eraseHandle : forall e1 e1' e2 e2' T, eraseTerm e1 T e1' -> eraseTerm e2 T e2' ->
+                                       eraseTerm (handle e1 e2) T (phandle e1' e2')
+|eraseDone : forall e e' T, eraseTerm e T e' -> eraseTerm (done e) T (pdone e')
+|eraseSpec : forall e1 e1' e2 e2' T i j, 
+               eraseTerm e1 T e1' -> eraseTerm e2 T e2' -> ~(appears_free_in i e2) ->
+               eraseTerm (spec e1 e2) T 
+   (pbind e1' (plambda i (pbind e2' (plambda j (pret (ppair (pvar i) (pvar j)))))))
+|eraseSpecReturn : forall e e' tid tid' tid'' T i j M M' M'' s1 s1' s2 , 
+                     eraseTerm e T e' -> s1 = s1' ++ [sAct tid'' M'] ->
+                     eraseTerm M' T M'' -> ~(appears_free_in i M') ->
+                     thread_lookup T tid (Some (thread tid' s1 s2 M)) ->
+                     eraseTerm (specReturn e (threadId tid)) T
+   (pbind e' (plambda i (pbind M'' (plambda j (pret (ppair (pvar i) (pvar j)))))))
+                                   
+.
+
+Hint Constructors eraseTerm. 
+
+Inductive eraseHeap : sHeap -> pHeap -> Prop :=
+|eraseSE : forall h h' (i:id) hd tl,
+             eraseHeap h h' -> eraseHeap ((i, empty (hd::tl)) :: h) h'
+|eraseCE : forall h h' i ,
+             eraseHeap h h' -> eraseHeap ((i, empty nil)::h) ((i, pempty)::h')
+|eraseSF : forall h h' i hd tl d s t N,
+             eraseHeap h h' -> eraseHeap ((i, full (hd::tl) d s t N)::h) h'
+|eraseCCSF : forall h h' i d hd tl t M,
+               eraseHeap h h' -> 
+               eraseHeap ((i, full nil d (hd::tl) t M)::h) ((i, pempty)::h')
+|eraseCCCF : forall h h' i d t M M',
+               eraseHeap h h' -> eraseTerm M dot M' ->
+               eraseHeap ((i, full nil d nil t M)::h) ((i, pfull M')::h')
+.
+
+Hint Constructors eraseHeap. 
+Inductive erasePool : pool -> pool -> ppool -> Prop :=
+|eraseDot : forall T, erasePool dot T pdot
+|erasePar : forall T1 T2 T1' T2' T,
+              erasePool T1 T T1' -> erasePool T2 T T2' ->
+              erasePool (par T1 T2) T (ppar T1' T2')
+|eraseCommitThread : forall tid s2 M M' T,
+                       eraseTerm M T M' -> 
+                       erasePool (thread tid nil s2 M) T (pthread M')
+|eraseThreadSR : forall tid tid' M M' M'' x s1 s2 s1' T,
+                   s1 = s1' ++ [rAct x tid' M'] -> eraseTerm M' T M'' ->
+                   erasePool (thread tid s1 s2 M) T (pthread M'')
+|eraseThreadSW : forall tid tid' M M' M'' x s1 s2 s1' T,
+                   s1 = s1' ++ [wAct x tid' M'] -> eraseTerm M' T M'' ->
+                   erasePool (thread tid s1 s2 M) T (pthread M'')
+|eraseThreadSC : forall tid tid' M M' M'' x s1 s2 s1' T,
+                   s1 = s1' ++ [cAct x tid' M'] -> eraseTerm M' T M'' ->
+                   erasePool (thread tid s1 s2 M) T (pthread M'')
+|eraseThreadSS : forall tid tid' M M' s1 s2 s1' T,
+                   s1 = s1' ++ [sAct tid' M'] -> 
+                   erasePool (thread tid s1 s2 M) T pdot
+|eraseThreadSF : forall tid tid' tid'' M M' M'' s1 s2 s1' T,
+                   s1 = s1' ++ [fAct tid' tid'' M'] -> eraseTerm M' T M'' ->
+                   erasePool (thread tid s1 s2 M) T (pthread M'')
+|eraseThreadJoin : forall tid M M' s1 s1' s2 T,
+                     s1 = s1' ++ [joinAct] -> eraseTerm M T M' ->
+                     erasePool (thread tid s1 s2 M) T (pthread M')
+|eraseThreadSpec : forall tid M s1 s1' s2 T,
+                     s1 = s1' ++ [specAct] -> 
+                     erasePool (thread tid s1 s2 M) T (pdot)
+.
+
+Hint Constructors erasePool. 
+
+Inductive Erase : sHeap -> pool -> pHeap -> ppool -> Prop :=
+  |erase : forall h t h' t', erasePool t t t' -> eraseHeap h h' ->
+                             Erase h t h' t'.
+
+Hint Constructors Erase. 
+
+Theorem eraseUnspecHeapIdem : 
+  forall H H' H'', unspecHeap H H' -> eraseHeap H' H'' -> eraseHeap H H''. 
+Proof. 
+  intros.   
+  {generalize dependent H''. 
+   induction H0; intros; try(solve[eauto]). 
+   {inversion H1; subst. apply IHunspecHeap in H4. constructor. assumption. }
+   {inversion H1; subst. apply IHunspecHeap in H4. constructor. assumption. }
+   {inversion H1; subst. apply IHunspecHeap in H7. constructor. assumption. 
+    assumption. }
+  }
+Qed. 
+
+Theorem Helper4 : 
+  forall P P', unspecT P P' -> 
+               forall tid, thread_lookup P' tid None ->
+                           thread_lookup P tid None.
+Proof.
+  intros. induction H; try(solve[eauto]);
+  try(inversion H0; subst; apply miss; assumption).  
+  {constructor. inversion H0; subst. apply IHunspecT1 in H4. 
+   assumption. inversion H0; subst. apply IHunspecT2 in H7. 
+   assumption. }
+Qed. 
+
+Theorem Helper3 : 
+  forall P P',
+    unspecT P P' -> forall tid T',
+    thread_lookup P' tid (Some T') -> 
+    exists T,thread_lookup P tid (Some T). 
+Proof. 
+  intros P P' H. induction H; intros. 
+  {inversion H. }
+  {inversion H1; subst. apply IHunspecT1 in H5. inversion H5. 
+   econstructor. constructor. eassumption. econstructor. 
+   apply IHunspecT2 in H7. inversion H7. eapply lookupPar2. 
+   eapply Helper4 in H. eassumption. assumption. eapply H2. 
+
+Theorem Helper3 : 
+  forall P P',
+    unspecT P P' -> forall tid T T',
+    thread_lookup P' tid (Some T') -> 
+    thread_lookup P tid (Some T). 
+Proof. 
+  intros P P' H. induction H; intros. 
+  {inversion H. }
+  {inversion H1; subst. eapply IHunspecT1 in H5. constructor. 
+   eassumption. eapply IHunspecT2 in H7. apply lookupPar2. 
+   eapply Helper4 in H. eassumption. eassumption. eassumption. }
+  {inversion H; subst. apply hit. 
 
 
 
+Theorem eraseHelper : 
+  forall M M' P P', unspecT P P' -> eraseTerm M P' M' -> eraseTerm M P M'.
+Proof.
+  intros. induction H0; try(solve[eauto]). 
+  {econstructor. apply IHeraseTerm1 in H. assumption. 
+   reflexivity. apply IHeraseTerm2 in H. eassumption. 
+   assumption. subst. 
+   eapply Helper3 with (tid := tid) 
+                         (T := (thread tid' (s1' ++ [sAct tid'' M']) s2 M)) 
+     in H. eassumption. eassumption. } 
+Qed. 
 
+
+
+Theorem eraseUnspecPoolIdem :
+  forall T T' T'' P P', unspecT P P' -> unspecT T T' -> erasePool T' P' T'' ->
+                        erasePool T P T''. 
+Proof. 
+  intros. generalize dependent P.  generalize dependent T''. 
+  dependent induction H0; try(solve[eauto]). 
+  {intros. inversion H1. constructor. }
+  {intros. inversion H1; subst. eapply IHunspecT1 in H3. 
+   eapply IHunspecT2 in H6. constructor; eassumption. assumption. assumption. }
+  {intros. inversion H1; subst. constructor. 
+
+
+
+Admitted. (*
+  {intros. admit. (* inversion H0; subst; try(destruct s1'0; inversion H7). 
+   econstructor. reflexivity. assumption.*) }
+  {intros. inversion H0; subst; try(destruct s1'0; inversion H7). 
+   eapply eraseThreadSW. reflexivity. assumption. }
+  {intros. inversion H0; subst; try(destruct s1'0; inversion H7). 
+   eapply eraseThreadSC. reflexivity. assumption. }
+  {intros. inversion H0; subst; destruct s1'0; inversion H7
+   ; try(destruct s1'0; inversion H2). subst. econstructor. 
+   reflexivity. }
+  {intros. inversion H0; subst; try(destruct s1'0; inversion H7). 
+   eapply eraseThreadSF. reflexivity. assumption. }
+Qed. *)
+
+Theorem ErasureUSIdempotence : 
+  forall H T H' T' H'' T'', unspec H T H' T' -> Erase H' T' H'' T'' ->
+                            Erase H T H'' T''. 
+Proof.
+  intros. inversion H0; subst. inversion H1; subst. 
+  constructor. eapply eraseUnspecPoolIdem in H3. 
+  eassumption. eassumption. eapply eraseUnspecHeapIdem in H2. 
+  eassumption. assumption. Qed. 
+  
