lvars/coq/Erasure.v
@@ -1,0 +1,50 @@
+Require Import Spec. 
+Require Import NonSpec. 
+
+Print unspecHeap. 
+
+Inductive eraseTerm : term -> pterm -> Prop :=
+.
+
+Inductive eraseHeap : sHeap -> pHeap -> Prop :=
+|eraseSE : forall h h' (i:id) hd tl,
+             eraseHeap h h' -> eraseHeap ((i, empty (hd::tl)) :: h) h'
+|eraseCE : forall h h' i ,
+             eraseHeap h h' -> eraseHeap ((i, empty nil)::h) ((i, pempty)::h')
+|eraseSF : forall h h' i hd tl d s t N,
+             eraseHeap h h' -> eraseHeap ((i, full (hd::tl) d s t N)::h) h'
+|eraseCCSF : forall h h' i d hd tl t M,
+               eraseHeap h h' -> 
+               eraseHeap ((i, full nil d (hd::tl) t M)::h) ((i, pempty)::h')
+|eraseCCCF : forall h h' i d t M M',
+               eraseHeap h h' -> eraseTerm M M' ->
+               eraseHeap ((i, full nil d nil t M)::h) ((i, pfull M')::h')
+.
+
+Print pool. 
+
+Print action. 
+
+Inductive erasePool : pool -> ppool -> Prop :=
+|erasePar : forall T1 T2 T1' T2',
+              erasePool T1 T1' -> erasePool T2 T2' ->
+              erasePool (par T1 T2) (ppar T1' T2')
+|eraseCommitThread : forall tid s2 M M',
+                       eraseTerm M M' -> erasePool (thread tid nil s2 M) (pthread M')
+|eraseThreadSR : forall tid tid' M M' M'' x s1 s2 s1',
+                   s1 = s1' ++ [rAct x tid' M'] -> eraseTerm M' M'' ->
+                   erasePool (thread tid s1 s2 M) (pthread M'')
+|eraseThreadSW : forall tid tid' M M' M'' x s1 s2 s1',
+                   s1 = s1' ++ [wAct x tid' M'] -> eraseTerm M' M'' ->
+                   erasePool (thread tid s1 s2 M) (pthread M'')
+|eraseThreadSC : forall tid tid' M M' M'' x s1 s2 s1',
+                   s1 = s1' ++ [cAct x tid' M'] -> eraseTerm M' M'' ->
+                   erasePool (thread tid s1 s2 M) (pthread M'')
+|eraseThreadSS : forall tid tid' M M' M'' s1 s2 s1',
+                   s1 = s1' ++ [sAct tid' M'] -> eraseTerm M' M'' ->
+                   erasePool (thread tid s1 s2 M) (pthread M'')
+.
+
+
+
+
