lvars/coq/Independence.v
@@ -1,49 +1,46 @@
 Require Import Spec. 
 Require Import Coq.Program.Equality. 
+Require Import SfLib. 
+
+Theorem listNeq : forall (T:Type) (h:T) l, l = h::l -> False. 
+Proof.
+  intros. induction l. 
+  {inversion H. }
+  {inversion H. apply IHl in H2. assumption. }
+Qed. 
+  
+Theorem listNeq2 : forall (T:Type) (h:T) t l, 
+                        h <> t -> h::l = l++[t] -> False. 
+Proof.
+  intros. induction l. 
+  {inversion H0. contradiction. }
+  {inversion H0. subst. apply IHl in H3. assumption. }
+Qed. 
+
+Theorem listNeq3 : forall (T:Type) (h:T) l, 
+                     l = l ++ [h] -> False. 
+Proof.
+  intros. induction l. 
+  {inversion H. }
+  {inversion H. apply IHl in H1. assumption. }
+Qed. 
+
 
 (*
-Theorem RBUntouched : 
-  forall tid H H' T1 T2 T2' T1', rollback tid H (par T1 T2) H' (par T1' T2) ->
-                                 rollback tid H (par T1 T2') H' (par T1' T2').
-Proof.
-  intros. apply rollback_ind. 
-  {intros. constructor. }
-  {intros. subst. eapply RBRead. reflexivity. eassumption. 
-   reflexivity. eassumption. }
-  {intros. subst. eapply RBFork. reflexivity. eassumption. }
-  {intros. subst. eapply RBWrite. reflexivity. eassumption. 
-   reflexivity. eassumption. }
-  {intros. subst. eapply RBNew. reflexivity. eassumption. 
-   reflexivity. eassumption. }
-  {intros. subst. eapply RBSpec. reflexivity. eassumption. }
-  {intros. apply RBCongr with (T' := T') (T'' := T''). 
-   assumption. assumption. assumption. }
-  *)
+IHrollback : forall T T', congr (par T1 T2') T -> congr T' (par T1' T2') ->
+                          rollback h T h' T'
+*)
 
-
-Theorem RBUntouched : 
-  forall tid H H' T1 T2 T2' T1', rollback tid H (par T1 T2) H' (par T1' T2) ->
-                                 rollback tid H (par T1 T2') H' (par T1' T2').
-Proof. intros. dependent induction H0; intros.  
-  {constructor. }
-  {eapply RBRead. reflexivity. eassumption. symmetry. reflexivity.  
-   assert((par (thread tid'' s1' s2 M') T2) = (par (thread tid'' s1' s2 M') T2)). 
-   reflexivity.  eapply IHrollback with (T1'0 := T1') in H. 
-   eassumption. reflexivity. }
-  {assert(par(thread tid'' s1' s2 M') T2 = par(thread tid'' s1' s2 M') T2). reflexivity. 
-   eapply IHrollback with (T1'0 := T1') in H. econstructor. reflexivity. 
-   eassumption. reflexivity. }
-  {assert(par (thread tid'' s1' s2 M') T2 = par (thread tid'' s1' s2 M') T2). 
-   reflexivity. eapply RBWrite. reflexivity. eassumption. 
-   reflexivity. eapply IHrollback with (T1'0 := T1') in H. 
-   eassumption. reflexivity. }
-  {eapply RBNew. reflexivity. eassumption. reflexivity. 
-   assert(par (thread tid'' s1' s2 M') T2 = par (thread tid'' s1' s2 M') T2 ). 
-   reflexivity. eapply IHrollback in H. eassumption. reflexivity. }
-  {eapply RBSpec. reflexivity. 
-   assert(par (thread tid'' s1' s2 M') T2 = par (thread tid'' s1' s2 M') T2). 
-   reflexivity. eapply IHrollback in H. eassumption. reflexivity. }
-  {admit. }
+Theorem RBUntouched : forall tid H H' T1 T2 T1', 
+                        rollback tid H (par T1 T2) H' (par T1' T2) ->
+                        forall T2',rollback tid H (par T1 T2') H' (par T1' T2').
+Proof. intros. dependent induction H0; eauto.  
+  {inversion H; subst. 
+   {inversion H0; subst. 
+    {admit. }
+    {admit. }
+    {
+  }
 Qed. 
 
 Theorem Reorder1Step3 : forall H T1 T2 H' T1' T2' sa ca,
@@ -53,28 +50,67 @@ Theorem Reorder1Step3 : forall H T1 T2 H' T1' T2' sa ca,
                          commitActions T2' ca -> 
                          step H (par T1 T2) H' (par T1' T2) ->
                          step H' (par T2 T1') H' (par T2' T1') -> 
-                         step H (par T2 T1) H (par T2' T1) /\ step H (par T1 T2') H' (par T1' T2'). 
-Proof.  
-  intros. dependent induction H5. 
-  {dependent induction H4; try(solve[try(repeat constructor; try(assumption; assumption); try subst);
-   try (solve[econstructor; try eassumption; try reflexivity])]). 
-   {constructor. constructor. assumption. reflexivity. 
-    apply Fork with (E := E0). assumption. reflexivity. }
-   {constructor. constructor. assumption. reflexivity. eapply PopSpec with (E := E0). 
-    assumption. reflexivity. reflexivity. }
-   {constructor. constructor. assumption. reflexivity. eapply SpecJoin with (E := E0).
-    assumption. reflexivity. }
+                         step H (par T2 T1) H (par T2' T1) /\ 
+                          step H (par T1 T2') H' (par T1' T2'). 
+Proof.   
+  intros. dependent induction H5.
+  {dependent induction H4; try(solve[eauto]). 
    {constructor. constructor. assumption. reflexivity. eapply SpecRB with (E := E0). 
-    assumption. reflexivity. apply RBUntouched with (T2' := (thread (bump tid) s1 s2 (E(app t2 t1)))) in H5. 
+    assumption. reflexivity. 
+    apply RBUntouched with (T2' := (thread (bump tid) s1 s2 (E(app t2 t1)))) in H5. 
     apply H5. }
-   {constructor. constructor. assumption. reflexivity. eapply SpecRaise with (E := E0). 
-    assumption. reflexivity. }
-   {constructor. constructor. assumption. reflexivity. eapply Handle with (E := E0). 
-    assumption. reflexivity. }
-   {constructor. constructor. assumption. reflexivity. eapply PopNewEmpty. 
-    reflexivity. eassumption. reflexivity. }
-   {constructor. constructor. assumption. reflexivity. eapply IHstep in H6. 
-    
+   {inversion H; subst; admit. }
+  }
+  {dependent induction H4; try(solve[eauto]). 
+   {constructor. econstructor. assumption. reflexivity. 
+    eapply SpecRB with (E := E0). assumption. reflexivity. 
+    apply RBUntouched with (T2' := (thread (bump tid)s1 s2) (E(raise M'))) in H5. 
+    eassumption. }
+   {admit. }
+  }
+  {dependent induction H4; try(solve[eauto]). 
+   {constructor. econstructor. eassumption. reflexivity. 
+    econstructor. assumption. reflexivity. eapply RBUntouched. eassumption. }
+   {admit. }
+  } 
+  {inversion H0. inversion H1. rewrite <- H12 in H5. inversion H5.
+   apply listNeq in H20. inversion H20. }
+  {inversion H0. inversion H1. subst sa. inversion H12. 
+   symmetry in H19. apply listNeq in H19. inversion H19. }
+  {inversion H0. inversion H1. inversion H13. inversion H15. 
+   subst. inversion H14. }
+  {inversion H0. inversion H1. inversion H13. inversion H15. 
+   inversion H8. inversion H10. subst. inversion H14. 
+   assert(joinAct <> sAct tid'' M). unfold not; intros. 
+   inversion H5. apply listNeq2 with (l := s1') in H5. 
+   inversion H5. assumption. }
+  {inversion H0. inversion H1. inversion H8. inversion H10. 
+   subst. inversion H9. }
+  {inversion H0. inversion H1. inversion H9. inversion H11. 
+   subst. inversion H10. }
+  {inversion H0. inversion H1. inversion H8. inversion H10. 
+   subst. inversion H9. }
+  {inversion H0. inversion H1. subst. inversion H12. 
+   symmetry in H10. apply listNeq in H10. inversion H10. }
+  {dependent induction H4; try(solve[eauto]). 
+   {constructor. eapply Handle. apply H6. reflexivity. 
+    econstructor. assumption. reflexivity. eapply RBUntouched. 
+    eassumption. }
+   {admit. }
+  }
+  {inversion H0. inversion H1. subst sa. inversion H11. 
+   apply listNeq3 in H18. inversion H18. }
+  {inversion H0. inversion H1. subst sa. inversion H11. 
+   apply listNeq3 in H18. inversion H18. }
+  {inversion H0. inversion H1. inversion H7. inversion H9.
+   inversion H12. inversion H14. subst. inversion H8. 
+   symmetry in H16. apply listNeq3 in H16. inversion H16. }
+  {inversion H0. inversion H1. subst sa. inversion H11. }
+  {admit. }
+Qed. 
+
+
+
 
 Theorem Reorder1Step2 : forall H T1 T2 H' T1' T2' sa ca,
                          specActions T2 sa -> 
